Expr -> expr, Stmt -> stmt.

src/ast.v
@@ -39,36 +39,36 @@ Inductive var: Type -> Type :=
 (*
  * expressions produce values
  *)
-Inductive Expr: Type -> Type :=
-| value: forall (t : Type), t -> Expr t
-| read: forall (t: Type), var t -> Expr t
-| cond: forall t, Expr bool -> Expr t -> Expr t -> Expr t
+Inductive expr: Type -> Type :=
+| value: forall (t : Type), t -> expr t
+| read: forall (t: Type), var t -> expr t
+| cond: forall t, expr bool -> expr t -> expr t -> expr t
 .
 
 (*
  * statements don't
  *)
-Inductive Stmt: Type :=
-| block: list Stmt -> Stmt
-| start: forall (pt : Type), Proc pt unit -> Expr pt -> Stmt
-| assign: forall t, var t -> Expr t -> Stmt
-| load: forall t, var t -> lock t -> Stmt
-| store: forall t, lock t -> Expr t -> Stmt
-| scope: Stmt -> Stmt
-| if_: Expr bool -> Stmt -> Stmt -> Stmt
-| while: Expr bool -> Stmt -> Stmt
-| call: forall (pt : Type) rt, var rt -> Proc pt rt -> Expr pt -> Stmt
-| local: forall t, var t -> Expr t -> Stmt
-| return_: forall t, Expr t -> Stmt
-| getlock: forall t, lock t -> Stmt
-| putlock: forall t, lock t -> Stmt
+Inductive stmt: Type :=
+| block: list stmt -> stmt
+| start: forall (pt : Type), Proc pt unit -> expr pt -> stmt
+| assign: forall t, var t -> expr t -> stmt
+| load: forall t, var t -> lock t -> stmt
+| store: forall t, lock t -> expr t -> stmt
+| scope: stmt -> stmt
+| if_: expr bool -> stmt -> stmt -> stmt
+| while: expr bool -> stmt -> stmt
+| call: forall (pt : Type) rt, var rt -> Proc pt rt -> expr pt -> stmt
+| local: forall t, var t -> expr t -> stmt
+| return_: forall t, expr t -> stmt
+| getlock: forall t, lock t -> stmt
+| putlock: forall t, lock t -> stmt
 with
 
 (*
  * procs both take and produce values
  *)
 (*Inductive*) Proc: Type -> Type -> Type :=
-| proc: forall pt rt, var pt -> Stmt -> Proc pt rt
+| proc: forall pt rt, var pt -> stmt -> Proc pt rt
 .
 
 
@@ -76,9 +76,9 @@ with
  * Extended/sugary AST forms
  *)
 
-Definition coqcall {ta tr : Set} (f : ta -> tr) (x : ta): Expr tr :=
+Definition coqcall {ta tr : Set} (f : ta -> tr) (x : ta): expr tr :=
    value tr (f x)
 .
 
-Definition skip: Stmt := block nil.
+Definition skip: stmt := block nil.
 
